progress: extend passification theory to handle old variables

BoogieLang/Passification.thy
@@ -57,31 +57,54 @@ proof (induction rule: red_expr_red_exprs.inducts)
     by simp
 qed (auto intro: red_expr_red_exprs.intros)
 
-(* todo: old variables, constants *)
-inductive expr_rel :: "passive_rel \<Rightarrow> expr \<Rightarrow> expr \<Rightarrow> bool" and 
- expr_list_rel :: "passive_rel \<Rightarrow> expr list \<Rightarrow> expr list \<Rightarrow> bool"
-  where    
-   Var_Rel: "R x1 = Some (Inl x2) \<Longrightarrow> expr_rel R (Var x1) (Var x2)"
- | Var_Const_Rel: "R x1 = Some (Inr l) \<Longrightarrow> expr_rel R (Var x1) (Lit l)"
- | BVar_Rel: "expr_rel R (BVar i) (BVar i)"
- | Lit_Rel: "expr_rel R (Lit lit) (Lit lit)"
- | UnOp_Rel: "expr_rel R e1 e2 \<Longrightarrow> expr_rel R (UnOp uop e1) (UnOp uop e2)"
- | BinOp_Rel: "\<lbrakk>expr_rel R e11 e21; expr_rel R e12 e22\<rbrakk> \<Longrightarrow> expr_rel R (e11 \<guillemotleft>bop\<guillemotright> e12) (e21 \<guillemotleft>bop\<guillemotright> e22)"
- | FunExp_Rel: "\<lbrakk>expr_list_rel R args1 args2 \<rbrakk>  \<Longrightarrow> expr_rel R (FunExp f ts args1) (FunExp f ts args2)"
-(* | OldExp_Rel: "expr_rel R (push_old_expr False (Old e1)) e2  \<Longrightarrow> expr_rel R (Old e1) e2" *)
- | Forall_Rel: "expr_rel R e1 e2 \<Longrightarrow> expr_rel R (Forall ty e1) (Forall ty e2)"
- | Exists_Rel: "expr_rel R e1 e2 \<Longrightarrow> expr_rel R (Exists ty e1) (Exists ty e2)"
- | ForallT_Rel: "expr_rel R e1 e2 \<Longrightarrow> expr_rel R (ForallT e1) (ForallT e2)"
- | ExistsT_Rel: "expr_rel R e1 e2 \<Longrightarrow> expr_rel R (ExistsT e1) (ExistsT e2)"
- | Nil_Rel: "expr_list_rel R [] []"
- | Cons_Rel: "expr_rel R x y \<Longrightarrow> expr_list_rel R xs ys \<Longrightarrow> expr_list_rel R (x#xs) (y#ys)"
+fun is_not_var :: "expr \<Rightarrow> bool"
+  where 
+    "is_not_var (Var _) = False"
+  | "is_not_var _ = True"
 
+
+text \<open> Expression relation \<close>
+text \<open> R: active variable relation, 
+       R_old: old global variable to passive variable relation, 
+       loc_vars: parameters and locals \<close>
+inductive expr_rel :: "passive_rel \<Rightarrow> passive_rel \<Rightarrow> vdecls \<Rightarrow> expr \<Rightarrow> expr \<Rightarrow> bool" and 
+ expr_list_rel :: "passive_rel \<Rightarrow> passive_rel \<Rightarrow> vdecls \<Rightarrow> expr list \<Rightarrow> expr list \<Rightarrow> bool"
+  for R :: passive_rel and R_old :: passive_rel and loc_vars :: vdecls
+  where    
+   Var_Rel: "R x1 = Some (Inl x2) \<Longrightarrow> expr_rel R R_old loc_vars (Var x1) (Var x2)"
+ | Var_Const_Rel: "R x1 = Some (Inr l) \<Longrightarrow> expr_rel R R_old loc_vars (Var x1) (Lit l)"
+ | BVar_Rel: "expr_rel R R_old loc_vars (BVar i) (BVar i)"
+ | Lit_Rel: "expr_rel R R_old loc_vars (Lit lit) (Lit lit)"
+ | UnOp_Rel: "expr_rel R R_old loc_vars e1 e2 \<Longrightarrow> expr_rel R R_old loc_vars (UnOp uop e1) (UnOp uop e2)"
+ | BinOp_Rel: "\<lbrakk> expr_rel R R_old loc_vars e11 e21; expr_rel R R_old loc_vars e12 e22 \<rbrakk> \<Longrightarrow> 
+              expr_rel R R_old loc_vars (e11 \<guillemotleft>bop\<guillemotright> e12) (e21 \<guillemotleft>bop\<guillemotright> e22)"
+ | FunExp_Rel: "\<lbrakk> expr_list_rel R R_old loc_vars args1 args2 \<rbrakk>  \<Longrightarrow> 
+              expr_rel R R_old loc_vars (FunExp f ts args1) (FunExp f ts args2)"
+ | OldGlobalVar_Rel: "\<lbrakk>R_old x = Some (Inl y)\<rbrakk> \<Longrightarrow>
+              expr_rel R R_old loc_vars (Old (Var x)) (Var y)"
+ | OldLocalVar_Rel: "\<lbrakk>map_of loc_vars x = Some v; expr_rel R R_old loc_vars (Var x) (Var y)\<rbrakk> \<Longrightarrow> 
+              expr_rel R R_old loc_vars (Old (Var x)) (Var y)"
+ | OldExp_Rel: "\<lbrakk> is_not_var e1; expr_rel R R_old loc_vars (push_old_expr False (Old e1)) e2 \<rbrakk>  \<Longrightarrow> 
+              expr_rel R R_old loc_vars (Old e1) e2"
+ | Forall_Rel: "\<lbrakk> expr_rel R R_old loc_vars e1 e2 \<rbrakk> \<Longrightarrow> 
+              expr_rel R R_old loc_vars (Forall ty e1) (Forall ty e2)"
+ | Exists_Rel: "\<lbrakk> expr_rel R R_old loc_vars e1 e2 \<rbrakk> \<Longrightarrow> 
+              expr_rel R R_old loc_vars (Exists ty e1) (Exists ty e2)"
+ | ForallT_Rel: "\<lbrakk> expr_rel R R_old loc_vars e1 e2 \<rbrakk> \<Longrightarrow> 
+              expr_rel R R_old loc_vars (ForallT e1) (ForallT e2)"
+ | ExistsT_Rel: "\<lbrakk> expr_rel R R_old loc_vars e1 e2 \<rbrakk> \<Longrightarrow> 
+             expr_rel R R_old loc_vars (ExistsT e1) (ExistsT e2)"
+ | Nil_Rel: "expr_list_rel R R_old loc_vars [] []"
+ | Cons_Rel: "\<lbrakk>expr_rel R R_old loc_vars x y; expr_list_rel R R_old loc_vars xs ys\<rbrakk> \<Longrightarrow>
+              expr_list_rel R R_old loc_vars (x#xs) (y#ys)"
+
+(*
 method expr_rel_tac uses R_def = 
   (match conclusion in "expr_rel ?R (Var ?x1) (Var ?x2)" \<Rightarrow> \<open>rule, solves \<open>simp add: R_def\<close>\<close> \<bar>
                        "expr_rel ?R ?e1 ?e2" \<Rightarrow> rule  \<bar>
                        "expr_list_rel ?R ?es1 ?es2" \<Rightarrow> rule \<bar> 
                        "_" \<Rightarrow> fail)+
-
+*)
 
 (* don't need to explicitly prove that constant has the declared type of the variable, since no 
 corresponding variable is constrained in the passive program *)
@@ -110,13 +133,22 @@ lemma rel_well_typed_update_const:
   unfolding rel_well_typed_def rel_const_correct_def
   by simp
 
+definition nstate_old_rel :: "var_context \<Rightarrow> var_context \<Rightarrow> passive_rel \<Rightarrow> 'a nstate \<Rightarrow> 'a nstate \<Rightarrow> bool"
+  where "nstate_old_rel \<Lambda> \<Lambda>' R ns1 ns2 = 
+          (\<forall>x y.  R x = Some (Inl y) \<longrightarrow> 
+                 (map_of (fst \<Lambda>) x \<noteq> None \<and> map_of (snd \<Lambda>) x = None) \<and>
+                 (\<exists>v. (old_global_state ns1) x = Some v \<and> lookup_var \<Lambda>' ns2 y = Some v))"
+
 definition nstate_rel :: "var_context \<Rightarrow> var_context \<Rightarrow> passive_rel \<Rightarrow> 'a nstate \<Rightarrow> 'a nstate \<Rightarrow> bool"
   where "nstate_rel \<Lambda> \<Lambda>' R ns1 ns2 = 
           ((\<forall>x y.  R x = Some (Inl y) \<longrightarrow> (lookup_var \<Lambda> ns1 x = lookup_var \<Lambda>' ns2 y))
             \<and> binder_state ns1 = binder_state ns2)"
 
-definition nstate_rel_states
+definition nstate_rel_states :: "var_context \<Rightarrow> var_context \<Rightarrow> passive_rel \<Rightarrow> 'a nstate \<Rightarrow> 'a nstate set \<Rightarrow> bool"
   where "nstate_rel_states \<Lambda> \<Lambda>' R ns U \<equiv> \<forall>u \<in> U. nstate_rel \<Lambda> \<Lambda>' R ns u"
+
+definition nstate_old_rel_states :: "var_context \<Rightarrow> var_context \<Rightarrow> passive_rel \<Rightarrow> 'a nstate \<Rightarrow> 'a nstate set \<Rightarrow> bool"
+  where "nstate_old_rel_states \<Lambda> \<Lambda>' R ns U \<equiv> \<forall>u \<in> U. nstate_old_rel \<Lambda> \<Lambda>' R ns u"
 
 lemma nstate_rel_update_const: "nstate_rel \<Lambda> \<Lambda>' R ns1 ns2 \<Longrightarrow> nstate_rel \<Lambda> \<Lambda>' (R(x \<mapsto> Inr l)) (update_var \<Lambda> ns1 x v) ns2"
   unfolding nstate_rel_def
@@ -187,73 +219,144 @@ lemma binder_update_nstate_rel: "nstate_rel \<Lambda> \<Lambda>' R ns1 ns2 \<Lon
   apply (simp only: lookup_full_ext_env_same)
   by (simp add: binder_full_ext_env_same)
 
+lemma binder_update_nstate_old_rel: "nstate_old_rel \<Lambda> \<Lambda>' R ns1 ns2 \<Longrightarrow> (\<And>v. nstate_old_rel \<Lambda> \<Lambda>' R (full_ext_env ns1 v) (full_ext_env ns2 v))"
+  unfolding nstate_old_rel_def
+  apply (simp only: lookup_full_ext_env_same)
+  by (simp add: binder_full_ext_env_same)
+
 lemma binder_update_rel_const: "rel_const_correct \<Lambda> R ns \<Longrightarrow> (\<And>v. rel_const_correct \<Lambda> R (full_ext_env ns v))"
   unfolding rel_const_correct_def
-  by (simp only: lookup_full_ext_env_same) auto    
+  by (simp only: lookup_full_ext_env_same) auto  
+
+lemma old_global_var_red:
+  assumes "A,\<Lambda>,\<Gamma>,\<Omega> \<turnstile> \<langle>Old (Var x),ns\<rangle> \<Down> v" and "map_of (snd \<Lambda>) x = None"
+  shows "v = the (old_global_state ns x)"
+  using assms
+  apply cases
+  by (auto split: option.split simp: lookup_var_def)
+
+lemma old_local_var_red_2:
+  assumes "A,\<Lambda>,\<Gamma>,\<Omega> \<turnstile> \<langle>Old (Var x),ns\<rangle> \<Down> v" and A2:"map_of (snd \<Lambda>) x \<noteq> None"
+  shows "v = the (local_state ns x)"
+  using assms
+  apply cases
+  apply (erule RedVar_case)
+  by (auto split: option.split simp: lookup_var_def)
+
+lemma old_local_var_red:
+  assumes "A,\<Lambda>,\<Gamma>,\<Omega> \<turnstile> \<langle>Old (Var x),ns\<rangle> \<Down> v" and A2:"map_of (snd \<Lambda>) x \<noteq> None"
+  shows "A,\<Lambda>,\<Gamma>,\<Omega> \<turnstile> \<langle>Var x,ns\<rangle> \<Down> v"
+ (* using old_local_var_red[OF assms] *)
+  using assms
+  apply cases
+  apply (erule RedVar_case)
+  by (metis RedVar lookup_var_def nstate.ext_inject nstate.surjective nstate.update_convs(2) option.case_eq_if)
+  
+(*
+lemma old_local_var_red:
+  assumes "A,\<Lambda>,\<Gamma>,\<Omega> \<turnstile> \<langle>Old (Var x),ns\<rangle> \<Down> v" and A2:"map_of (fst \<Lambda>) x = None"
+  shows "v = the (local_state ns x)"
+  using assms
+  apply cases
+  apply (erule RedVar_case)
+  unfolding lookup_var_def
+  apply (auto split: option.split)
+*)
 
 lemma expr_rel_same:
-  shows "expr_rel R e1 e2 \<Longrightarrow> rel_const_correct \<Lambda> R ns1 \<Longrightarrow> nstate_rel \<Lambda> \<Lambda>' R ns1 ns2 \<Longrightarrow> A,\<Lambda>,\<Gamma>,\<Omega> \<turnstile> \<langle>e1, ns1\<rangle> \<Down> v \<Longrightarrow> A,\<Lambda>',\<Gamma>,\<Omega> \<turnstile> \<langle>e2, ns2\<rangle> \<Down> v" and
-    "expr_list_rel R es1 es2 \<Longrightarrow> rel_const_correct \<Lambda> R ns1 \<Longrightarrow> nstate_rel \<Lambda> \<Lambda>' R ns1 ns2 \<Longrightarrow> A,\<Lambda>,\<Gamma>,\<Omega> \<turnstile> \<langle>es1, ns1\<rangle> [\<Down>] vs \<Longrightarrow> A,\<Lambda>',\<Gamma>,\<Omega> \<turnstile> \<langle>es2, ns2\<rangle> [\<Down>] vs" 
+  shows "expr_rel R R_old (snd \<Lambda>) e1 e2 \<Longrightarrow>
+         rel_const_correct \<Lambda> R ns1 \<Longrightarrow> 
+         nstate_rel \<Lambda> \<Lambda>' R ns1 ns2 \<Longrightarrow> 
+         nstate_old_rel \<Lambda> \<Lambda>' R_old ns1 ns2 \<Longrightarrow>
+         A,\<Lambda>,\<Gamma>,\<Omega> \<turnstile> \<langle>e1, ns1\<rangle> \<Down> v \<Longrightarrow> 
+         A,\<Lambda>',\<Gamma>,\<Omega> \<turnstile> \<langle>e2, ns2\<rangle> \<Down> v" and
+    "expr_list_rel R R_old (snd \<Lambda>) es1 es2 \<Longrightarrow>
+     rel_const_correct \<Lambda> R ns1 \<Longrightarrow> 
+     nstate_rel \<Lambda> \<Lambda>' R ns1 ns2 \<Longrightarrow> 
+     nstate_old_rel \<Lambda> \<Lambda>' R_old ns1 ns2 \<Longrightarrow>
+     A,\<Lambda>,\<Gamma>,\<Omega> \<turnstile> \<langle>es1, ns1\<rangle> [\<Down>] vs \<Longrightarrow> 
+     A,\<Lambda>',\<Gamma>,\<Omega> \<turnstile> \<langle>es2, ns2\<rangle> [\<Down>] vs" 
 proof (induction arbitrary: v ns1 ns2 \<Omega> and vs ns1 ns2 \<Omega> rule: expr_rel_expr_list_rel.inducts)
-  case (Var_Rel R x1 x2)
+next
+  case (OldGlobalVar_Rel x y)  
+  from \<open>R_old x = Some (Inl y)\<close> and \<open>nstate_old_rel \<Lambda> \<Lambda>' R_old ns1 ns2\<close>
+  show ?case using old_global_var_red[OF \<open>A,\<Lambda>,\<Gamma>,\<Omega> \<turnstile> \<langle>Old (Var x),ns1\<rangle> \<Down> v\<close>]
+    by (metis RedVar nstate_old_rel_def option.sel)
+next
+  case (OldLocalVar_Rel x v')
+  thus ?case
+    using old_local_var_red[OF \<open> A,\<Lambda>,\<Gamma>,\<Omega> \<turnstile> \<langle>Old (Var x),ns1\<rangle> \<Down> v\<close>] \<open>map_of (snd \<Lambda>) x = Some v'\<close>
+    by auto   
+next
+  case (OldExp_Rel e1 e2)
+  thus ?case
+    using push_old_false_same by blast
+next
+  case (Var_Rel x1 x2)
   thus ?case  by (auto intro: red_expr_red_exprs.intros simp: nstate_rel_def)
 next
-  case (Var_Const_Rel R x1 l)
+  case (Var_Const_Rel x1 l)
   then show ?case by (auto intro: red_expr_red_exprs.intros simp: rel_const_correct_def)
 next
-  case (BVar_Rel R x1 x2)
+  case (BVar_Rel x1 x2)
   thus ?case 
  by (auto intro: red_expr_red_exprs.intros simp: nstate_rel_def)
 next
-  case (Lit_Rel R lit)
+  case (Lit_Rel lit)
   then show ?case by (blast intro: red_expr_red_exprs.intros )
 next
-  case (UnOp_Rel R e1 e2 uop)
+  case (UnOp_Rel e1 e2 uop)
   then show ?case by (blast intro: red_expr_red_exprs.intros)
 next
-  case (BinOp_Rel R e11 e21 e12 e22 bop)
+  case (BinOp_Rel e11 e21 e12 e22 bop)
   then show ?case by (blast intro: red_expr_red_exprs.intros)
 next
-  case (FunExp_Rel R args1 args2 f ts)
+  case (FunExp_Rel args1 args2 f ts)
   then show ?case by (blast intro: red_expr_red_exprs.intros)
 next
-  case (Forall_Rel R e1 e2 ty)
-  hence RelExt:"\<And>v. nstate_rel \<Lambda> \<Lambda>' R (full_ext_env ns1 v) (full_ext_env ns2 v)" using binder_update_nstate_rel by blast 
-  from Forall_Rel have RelWtExt:"\<And>v. rel_const_correct \<Lambda> R (full_ext_env ns1 v)" using binder_update_rel_const by blast 
-  from \<open>A,\<Lambda>,\<Gamma>,\<Omega> \<turnstile> \<langle>Forall ty e1,ns1\<rangle> \<Down> v\<close>
-  show ?case
-  by (cases; blast intro: red_expr_red_exprs.intros dest:Forall_Rel.IH[OF RelWtExt RelExt])
-next
-  case (Exists_Rel R e1 e2 ty)
+  case (Forall_Rel e1 e2 ty)
   hence RelExt:"\<And>v. nstate_rel \<Lambda> \<Lambda>' R (full_ext_env ns1 v) (full_ext_env ns2 v)" using binder_update_nstate_rel by blast
+  from Forall_Rel have RelOldExt: "\<And>v. nstate_old_rel \<Lambda> \<Lambda>' R_old (full_ext_env ns1 v) (full_ext_env ns2 v)" using binder_update_nstate_old_rel by blast 
+  from Forall_Rel have RelWtExt:"\<And>v. rel_const_correct \<Lambda> R (full_ext_env ns1 v)" using binder_update_rel_const by blast   
+  from \<open>A,\<Lambda>,\<Gamma>,\<Omega> \<turnstile> \<langle>Forall ty e1,ns1\<rangle> \<Down> v\<close>     
+  show ?case
+    by (cases; blast intro: red_expr_red_exprs.intros dest:Forall_Rel.IH(2)[OF RelWtExt RelExt RelOldExt])
+next
+  case (Exists_Rel e1 e2 ty)
+  hence RelExt:"\<And>v. nstate_rel \<Lambda> \<Lambda>' R (full_ext_env ns1 v) (full_ext_env ns2 v)" using binder_update_nstate_rel by blast
+  from Exists_Rel have RelOldExt: "\<And>v. nstate_old_rel \<Lambda> \<Lambda>' R_old (full_ext_env ns1 v) (full_ext_env ns2 v)" using binder_update_nstate_old_rel by blast 
   from Exists_Rel have RelWtExt:"\<And>v. rel_const_correct \<Lambda> R (full_ext_env ns1 v)" using binder_update_rel_const by blast 
   from \<open>A,\<Lambda>,\<Gamma>,\<Omega> \<turnstile> \<langle>Exists ty e1,ns1\<rangle> \<Down> v\<close>
   show ?case
-    by (cases; blast intro: red_expr_red_exprs.intros dest:Exists_Rel.IH[OF RelWtExt RelExt])
+    by (cases; blast intro: red_expr_red_exprs.intros dest:Exists_Rel.IH(2)[OF RelWtExt RelExt RelOldExt])
 next
-  case (ForallT_Rel R e1 e2)
+  case (ForallT_Rel e1 e2)
   from \<open>A,\<Lambda>,\<Gamma>,\<Omega> \<turnstile> \<langle>ForallT e1,ns1\<rangle> \<Down> v\<close>
   show ?case
-    by cases (auto intro: red_expr_red_exprs.intros dest: ForallT_Rel.IH[OF \<open>rel_const_correct \<Lambda> R ns1\<close> \<open>nstate_rel \<Lambda> \<Lambda>' R ns1 ns2\<close>])
+    by cases (auto intro: red_expr_red_exprs.intros dest: ForallT_Rel.IH(2)[OF \<open>rel_const_correct \<Lambda> R ns1\<close> \<open>nstate_rel \<Lambda> \<Lambda>' R ns1 ns2\<close> \<open>nstate_old_rel \<Lambda> \<Lambda>' R_old ns1 ns2\<close>])
 next
-  case (ExistsT_Rel R e1 e2)
+  case (ExistsT_Rel e1 e2)
   from \<open>A,\<Lambda>,\<Gamma>,\<Omega> \<turnstile> \<langle>ExistsT e1,ns1\<rangle> \<Down> v\<close>
   show ?case
-    by cases (auto intro: red_expr_red_exprs.intros dest: ExistsT_Rel.IH[OF \<open>rel_const_correct \<Lambda> R ns1\<close> \<open>nstate_rel \<Lambda> \<Lambda>' R ns1 ns2\<close>])
+    by cases (auto intro: red_expr_red_exprs.intros dest: ExistsT_Rel.IH(2)[OF \<open>rel_const_correct \<Lambda> R ns1\<close> \<open>nstate_rel \<Lambda> \<Lambda>' R ns1 ns2\<close> \<open>nstate_old_rel \<Lambda> \<Lambda>' R_old ns1 ns2\<close>])
 next
-  case (Nil_Rel R)
+  case Nil_Rel
   then show ?case
     using RedExpListNil by blast 
 next
-  case (Cons_Rel R x y xs ys)
+  case (Cons_Rel x y xs ys)
   thus ?case
     by (blast elim: cons_exp_elim2 intro: red_expr_red_exprs.intros)
 qed
 
 lemma expr_rel_same_set:
-  assumes "expr_rel R e1 e2" and "A,\<Lambda>,\<Gamma>,\<Omega> \<turnstile> \<langle>e1, ns1\<rangle> \<Down> v" and "rel_const_correct \<Lambda> R ns1" and "nstate_rel_states \<Lambda> \<Lambda>' R ns1 U"
+  assumes "expr_rel R R_old (snd \<Lambda>) e1 e2" and 
+          "A,\<Lambda>,\<Gamma>,\<Omega> \<turnstile> \<langle>e1, ns1\<rangle> \<Down> v" and 
+          "rel_const_correct \<Lambda> R ns1" and
+          "nstate_rel_states \<Lambda> \<Lambda>' R ns1 U" and
+          "nstate_old_rel_states \<Lambda> \<Lambda>' R_old ns1 U"
   shows "\<forall>u \<in> U. A,\<Lambda>',\<Gamma>,\<Omega> \<turnstile> \<langle>e2, u\<rangle> \<Down> v"
-  using assms expr_rel_same unfolding nstate_rel_states_def by blast
+  using assms expr_rel_same unfolding nstate_rel_states_def nstate_old_rel_states_def by blast
 
 fun varsInExpr :: "expr \<Rightarrow> vname set"
   where
@@ -421,10 +524,11 @@ proof (unfold nstate_rel_states_def, rule ballI)
 qed
 
 lemma assume_assign_nstate_rel:
-  assumes Erel:"expr_rel R e1 e2" and
+  assumes Erel:"expr_rel R R_old (snd \<Lambda>) e1 e2" and
           "A,\<Lambda>,\<Gamma>,\<Omega> \<turnstile> \<langle>e1, ns\<rangle> \<Down> v" and
-          Srel:"nstate_rel_states \<Lambda> \<Lambda>' R ns U" and 
-          Crel:"rel_const_correct \<Lambda> R ns"
+          Rel:"nstate_rel_states \<Lambda> \<Lambda>' R ns U" and
+          OldRel: "nstate_old_rel_states \<Lambda> \<Lambda>' R_old ns U" and
+          CRel:"rel_const_correct \<Lambda> R ns"
   shows   "nstate_rel_states 
                \<Lambda> \<Lambda>' (R(x_orig \<mapsto> (Inl x))) (update_var \<Lambda> ns x_orig v) {ns'. Normal ns' \<in> (set_red_cmd A M \<Lambda>' \<Gamma> \<Omega> (Assume ((Var x) \<guillemotleft>Eq\<guillemotright> e2)) U)}" 
  (is "nstate_rel_states \<Lambda> \<Lambda>' (R(x_orig \<mapsto> (Inl x))) (update_var \<Lambda> ns x_orig v) ?U'")
@@ -433,8 +537,9 @@ proof (unfold nstate_rel_states_def, rule ballI)
   fix u'
   assume "u' \<in> ?U'"
   hence "u' \<in> U" using passive_states_subset[OF Apassive] by blast
-  with Srel have "nstate_rel \<Lambda> \<Lambda>' R ns u'" by (simp add: nstate_rel_states_def)
-  have "A,\<Lambda>',\<Gamma>,\<Omega> \<turnstile> \<langle>e2, u'\<rangle> \<Down> v" using expr_rel_same(1)[OF Erel Crel \<open>nstate_rel \<Lambda> \<Lambda>' R ns u'\<close> \<open>A,\<Lambda>,\<Gamma>,\<Omega> \<turnstile> \<langle>e1, ns\<rangle> \<Down> v\<close>] by simp
+  with Rel have Rel2:"nstate_rel \<Lambda> \<Lambda>' R ns u'" by (simp add: nstate_rel_states_def)
+  from \<open>u' \<in> U\<close> and OldRel have OldRel2:"nstate_old_rel \<Lambda> \<Lambda>' R_old ns u'" by (simp add: nstate_old_rel_states_def)
+  have "A,\<Lambda>',\<Gamma>,\<Omega> \<turnstile> \<langle>e2, u'\<rangle> \<Down> v" using expr_rel_same(1)[OF Erel CRel Rel2 OldRel2 \<open>A,\<Lambda>,\<Gamma>,\<Omega> \<turnstile> \<langle>e1, ns\<rangle> \<Down> v\<close>] by simp
   from \<open>u' \<in> ?U'\<close> have "A,\<Lambda>',\<Gamma>,\<Omega> \<turnstile> \<langle>Var x, u'\<rangle> \<Down> v" 
      using  expr_eval_determ(1)[OF \<open>A,\<Lambda>',\<Gamma>,\<Omega> \<turnstile> \<langle>e2, u'\<rangle> \<Down> v\<close>] assume_reduction_args by metis
   hence "lookup_var \<Lambda>' u' x = Some v" by auto
@@ -454,13 +559,15 @@ lemma single_assign_reduce_2:
 lemma assume_rel_normal:
   assumes Ared:"A,\<Lambda>,\<Gamma>,\<Omega> \<turnstile> \<langle>e1, ns\<rangle> \<Down> (BoolV True)" and
           Srel:"nstate_rel_states \<Lambda> \<Lambda>' R ns U" and 
+          OldRel: "nstate_old_rel_states \<Lambda> \<Lambda>' R_old ns U" and
           Crel:"rel_const_correct \<Lambda> R ns" and
-          Erel:"expr_rel R e1 e2"
+          Erel:"expr_rel R R_old (snd \<Lambda>) e1 e2"
         shows "\<And>u. u \<in> U \<Longrightarrow> A,M,\<Lambda>',\<Gamma>,\<Omega> \<turnstile> \<langle>Assume e2, Normal u\<rangle> \<rightarrow> Normal u"
 proof -
   fix u
   assume "u \<in> U"
-  with Srel have "nstate_rel \<Lambda> \<Lambda>' R ns u" by (simp add: nstate_rel_states_def)
+  with Srel OldRel have "nstate_rel \<Lambda> \<Lambda>' R ns u" and "nstate_old_rel \<Lambda> \<Lambda>' R_old ns u"    
+      by (auto simp:  nstate_rel_states_def nstate_old_rel_states_def)
   with Ared Erel have "A,\<Lambda>',\<Gamma>,\<Omega> \<turnstile> \<langle>e2, u\<rangle> \<Down> (BoolV True)" using expr_rel_same Crel by blast
   thus "A,M,\<Lambda>',\<Gamma>,\<Omega> \<turnstile> \<langle>Assume e2,Normal u\<rangle> \<rightarrow> Normal u" by (auto intro: RedAssumeOk)
 qed
@@ -468,13 +575,15 @@ qed
 lemma assume_rel_magic:
   assumes Ared:"A,\<Lambda>,\<Gamma>,\<Omega> \<turnstile> \<langle>e1, ns\<rangle> \<Down> (BoolV False)" and
           Srel:"nstate_rel_states \<Lambda> \<Lambda>' R ns U" and
+          OldRel: "nstate_old_rel_states \<Lambda> \<Lambda>' R_old ns U" and
           Crel:"rel_const_correct \<Lambda> R ns" and
-          Erel:"expr_rel R e1 e2"
+          Erel:"expr_rel R R_old (snd \<Lambda>) e1 e2"
   shows "\<And>u. u \<in> U \<Longrightarrow> A,M,\<Lambda>',\<Gamma>,\<Omega> \<turnstile> \<langle>Assume e2, Normal u\<rangle> \<rightarrow> Magic"
 proof -
   fix u
   assume "u \<in> U"
-  with Srel have "nstate_rel \<Lambda> \<Lambda>' R ns u" by (simp add: nstate_rel_states_def)
+  with Srel OldRel have "nstate_rel \<Lambda> \<Lambda>' R ns u" and "nstate_old_rel \<Lambda> \<Lambda>' R_old ns u"    
+    by (auto simp:  nstate_rel_states_def nstate_old_rel_states_def)
   with Ared Erel have "A,\<Lambda>',\<Gamma>,\<Omega> \<turnstile> \<langle>e2, u\<rangle> \<Down> (BoolV False)" using expr_rel_same Crel by blast
   thus "A,M,\<Lambda>',\<Gamma>,\<Omega> \<turnstile> \<langle>Assume e2,Normal u\<rangle> \<rightarrow> Magic" by (auto intro: RedAssumeMagic)
 qed
@@ -482,8 +591,9 @@ qed
 lemma assert_rel_normal:
   assumes Ared:"A,\<Lambda>,\<Gamma>,\<Omega> \<turnstile> \<langle>e1, ns\<rangle> \<Down> (BoolV True)" and
           Srel:"nstate_rel_states \<Lambda> \<Lambda>' R ns U" and 
+          OldRel: "nstate_old_rel_states \<Lambda> \<Lambda>' R_old ns U" and
           Crel:"rel_const_correct \<Lambda> R ns" and
-          Erel:"expr_rel R e1 e2"
+          Erel:"expr_rel R R_old (snd \<Lambda>) e1 e2"
   shows "{ns'. Normal ns' \<in> (set_red_cmd A M \<Lambda>' \<Gamma> \<Omega> (Assert e2) U)} = U" (is "?U' = U")
 proof 
   have Apassive:"isPassive (Assert e2)" by simp
@@ -493,7 +603,8 @@ next
   proof
     fix u
     assume "u \<in> U"
-    with Srel have "nstate_rel \<Lambda> \<Lambda>' R ns u" by (simp add: nstate_rel_states_def)
+    with Srel OldRel have "nstate_rel \<Lambda> \<Lambda>' R ns u" and "nstate_old_rel \<Lambda> \<Lambda>' R_old ns u"    
+      by (auto simp:  nstate_rel_states_def nstate_old_rel_states_def)
     with Ared Erel have "A,\<Lambda>',\<Gamma>,\<Omega> \<turnstile> \<langle>e2, u\<rangle> \<Down> (BoolV True)" using expr_rel_same Crel by blast
     with \<open>u \<in> U\<close> show "u \<in> ?U'"
       by (auto intro!: red_cmd.intros simp: set_red_cmd_def)
@@ -503,27 +614,31 @@ qed
 lemma assert_rel_normal_2:
   assumes Ared:"A,\<Lambda>,\<Gamma>,\<Omega> \<turnstile> \<langle>e1, ns\<rangle> \<Down> (BoolV True)" and
           Srel:"nstate_rel_states \<Lambda> \<Lambda>' R ns U" and
+          OldRel: "nstate_old_rel_states \<Lambda> \<Lambda>' R_old ns U" and
           Crel:"rel_const_correct \<Lambda> R ns" and
-          Erel:"expr_rel R e1 e2"
+          Erel:"expr_rel R R_old (snd \<Lambda>) e1 e2"
         shows "\<And>u. u \<in> U \<Longrightarrow> A,M,\<Lambda>',\<Gamma>,\<Omega> \<turnstile> \<langle>Assert e2, Normal u\<rangle> \<rightarrow> Normal u"
 proof -
   fix u
   assume "u \<in> U"
-  with Srel have "nstate_rel \<Lambda> \<Lambda>' R ns u" by (simp add: nstate_rel_states_def)
+  with Srel OldRel have "nstate_rel \<Lambda> \<Lambda>' R ns u" and "nstate_old_rel \<Lambda> \<Lambda>' R_old ns u"    
+    by (auto simp:  nstate_rel_states_def nstate_old_rel_states_def)
   with Ared Erel have "A,\<Lambda>',\<Gamma>,\<Omega> \<turnstile> \<langle>e2, u\<rangle> \<Down> (BoolV True)" using expr_rel_same Crel by blast
   thus "A,M,\<Lambda>',\<Gamma>,\<Omega> \<turnstile> \<langle>Assert e2,Normal u\<rangle> \<rightarrow> Normal u" by (auto intro: RedAssertOk)
 qed
 
 lemma assert_rel_failure:
   assumes Ared:"A,\<Lambda>,\<Gamma>,\<Omega> \<turnstile> \<langle>e1, ns\<rangle> \<Down> (BoolV False)" and
-          Srel:"nstate_rel_states \<Lambda> \<Lambda>' R ns U" and 
+          Srel:"nstate_rel_states \<Lambda> \<Lambda>' R ns U" and
+          OldRel: "nstate_old_rel_states \<Lambda> \<Lambda>' R_old ns U" and
           Crel:"rel_const_correct \<Lambda> R ns" and
-          Erel:"expr_rel R e1 e2"
+          Erel:"expr_rel R R_old (snd \<Lambda>) e1 e2"
   shows "\<And>u. u \<in> U \<Longrightarrow> A,M,\<Lambda>',\<Gamma>,\<Omega> \<turnstile> \<langle>Assert e2, Normal u\<rangle> \<rightarrow> Failure"
 proof -
   fix u
   assume "u \<in> U"
-  with Srel have "nstate_rel \<Lambda> \<Lambda>' R ns u" by (simp add: nstate_rel_states_def)
+  with Srel OldRel have "nstate_rel \<Lambda> \<Lambda>' R ns u" and "nstate_old_rel \<Lambda> \<Lambda>' R_old ns u"    
+      by (auto simp:  nstate_rel_states_def nstate_old_rel_states_def)
   with Ared Erel have "A,\<Lambda>',\<Gamma>,\<Omega> \<turnstile> \<langle>e2, u\<rangle> \<Down> (BoolV False)" using expr_rel_same Crel by blast
   thus "A,M,\<Lambda>',\<Gamma>,\<Omega> \<turnstile> \<langle>Assert e2,Normal u\<rangle> \<rightarrow> Failure" by (auto intro: RedAssertFail)
 qed
@@ -562,28 +677,30 @@ definition passive_sim
                        (\<forall>ns'. s' = Normal ns' \<longrightarrow> (su = Normal u \<and> nstate_rel \<Lambda> \<Lambda>' R ns' u \<and> rel_well_typed A \<Lambda> \<Omega> R ns')))"
 
 
-inductive passive_cmds_rel :: "vname list \<Rightarrow> passive_rel \<Rightarrow> (vname \<times> (vname + lit)) list \<Rightarrow> cmd list \<Rightarrow> cmd list \<Rightarrow> bool"
+inductive passive_cmds_rel :: "vdecls \<Rightarrow> vname list \<Rightarrow> passive_rel \<Rightarrow> passive_rel \<Rightarrow> (vname \<times> (vname + lit)) list \<Rightarrow> cmd list \<Rightarrow> cmd list \<Rightarrow> bool"
+  for loc_vars :: vdecls
   where 
     PAssignNormal: 
-    "\<lbrakk> expr_rel R e1 e2; passive_cmds_rel W (R(x1 \<mapsto> (Inl x2))) Q cs1 cs2 \<rbrakk> \<Longrightarrow> 
-        passive_cmds_rel (x2#W) R ((x1,(Inl x2))#Q) ((Assign x1 e1) # cs1) ((Assume ((Var x2) \<guillemotleft>Eq\<guillemotright> e2)) # cs2)"
+    "\<lbrakk> expr_rel R R_old loc_vars e1 e2; passive_cmds_rel loc_vars W (R(x1 \<mapsto> (Inl x2))) R_old Q cs1 cs2 \<rbrakk> \<Longrightarrow> 
+        passive_cmds_rel loc_vars (x2#W) R R_old ((x1,(Inl x2))#Q) ((Assign x1 e1) # cs1) ((Assume ((Var x2) \<guillemotleft>Eq\<guillemotright> e2)) # cs2)"
   | PConst:
-    " \<lbrakk> passive_cmds_rel W (R(x1 \<mapsto> (Inr l))) Q cs1 cs2 \<rbrakk> \<Longrightarrow>
-       passive_cmds_rel W R ((x1, (Inr l))#Q) ((Assign x1 (Lit l))#cs1) cs2"
+    " \<lbrakk> passive_cmds_rel loc_vars W (R(x1 \<mapsto> (Inr l))) R_old Q cs1 cs2 \<rbrakk> \<Longrightarrow>
+       passive_cmds_rel loc_vars W R R_old ((x1, (Inr l))#Q) ((Assign x1 (Lit l))#cs1) cs2"
   | PAssert: 
-    "\<lbrakk> expr_rel R e1 e2; passive_cmds_rel W R Q cs1 cs2 \<rbrakk> \<Longrightarrow> 
-        passive_cmds_rel W R Q ((Assert e1) # cs1) ((Assert e2) # cs2)"
+    "\<lbrakk> expr_rel R R_old loc_vars e1 e2; passive_cmds_rel loc_vars W R R_old Q cs1 cs2 \<rbrakk> \<Longrightarrow> 
+        passive_cmds_rel loc_vars W R R_old Q ((Assert e1) # cs1) ((Assert e2) # cs2)"
   | PAssumeNormal: 
-    "\<lbrakk> expr_rel R e1 e2; passive_cmds_rel W R Q cs1 cs2 \<rbrakk> \<Longrightarrow> 
-        passive_cmds_rel W R Q ((Assume e1) # cs1) ((Assume e2) # cs2)"
+    "\<lbrakk> expr_rel R R_old loc_vars e1 e2; passive_cmds_rel loc_vars W R R_old Q cs1 cs2 \<rbrakk> \<Longrightarrow> 
+        passive_cmds_rel loc_vars W R R_old Q ((Assume e1) # cs1) ((Assume e2) # cs2)"
   | PHavoc: 
-    "\<lbrakk> passive_cmds_rel W (R(x \<mapsto> (Inl x'))) Q cs1 cs2\<rbrakk> \<Longrightarrow> 
-       passive_cmds_rel (x'#W) R ((x,(Inl x'))#Q) ((Havoc x) # cs1) cs2"
+    "\<lbrakk> passive_cmds_rel loc_vars W (R(x \<mapsto> (Inl x'))) R_old Q cs1 cs2\<rbrakk> \<Longrightarrow> 
+       passive_cmds_rel loc_vars (x'#W) R R_old ((x,(Inl x'))#Q) ((Havoc x) # cs1) cs2"
   | PSync:       
-    "\<lbrakk> R x = Some (Inl x1); passive_cmds_rel W (R(x \<mapsto> (Inl x2))) Q [] cs \<rbrakk> \<Longrightarrow>
-       passive_cmds_rel (x2#W) R ((x,(Inl x2))#Q) [] ((Assume ( (Var x2) \<guillemotleft>Eq\<guillemotright> (Var x1))) # cs)"
-  | PNil: "passive_cmds_rel [] R [] [] []"
+    "\<lbrakk> R x = Some (Inl x1); passive_cmds_rel loc_vars W (R(x \<mapsto> (Inl x2))) R_old Q [] cs \<rbrakk> \<Longrightarrow>
+       passive_cmds_rel loc_vars (x2#W) R R_old ((x,(Inl x2))#Q) [] ((Assume ( (Var x2) \<guillemotleft>Eq\<guillemotright> (Var x1))) # cs)"
+  | PNil: "passive_cmds_rel loc_vars [] R R_old [] [] []"
 
+(*
 method passive_rel_tac uses R_def = 
   (match conclusion in
                        "passive_cmds_rel ?W ?R ?Q [] []" \<Rightarrow> \<open>rule PNil\<close> \<bar>
@@ -591,6 +708,7 @@ method passive_rel_tac uses R_def =
                        "passive_cmds_rel ?W ?R ?Q [] ?cs2" \<Rightarrow> \<open>rule PSync, solves \<open>simp add: R_def\<close>\<close>  \<bar>
                        "passive_cmds_rel ?W ?R ?Q ?cs1 ?cs2" \<Rightarrow> \<open>rule, solves \<open>expr_rel_tac R_def: R_def\<close>\<close> \<bar>                 
                        "_" \<Rightarrow> fail)+
+*)
 
 (* "semantic" block lemma *)
 (*
@@ -618,10 +736,11 @@ definition type_rel :: "var_context \<Rightarrow> var_context \<Rightarrow> (vna
 (* helper lemma to prove semantic block lemma *)
 lemma passification_block_lemma_aux:
   assumes 
-          "passive_cmds_rel W R Q cs1 cs2" and
+          "passive_cmds_rel (snd \<Lambda>) W R R_old Q cs1 cs2" and
           "A,M,\<Lambda>,\<Gamma>,\<Omega> \<turnstile> \<langle>cs1, Normal ns\<rangle> [\<rightarrow>] s'" and          
           "dependent A \<Lambda>' \<Omega> U0 D0" and
           "nstate_rel_states \<Lambda> \<Lambda>' R ns U0" and
+          "nstate_old_rel_states \<Lambda> \<Lambda>' R_old ns U0" and
           "rel_well_typed A \<Lambda> \<Omega> R ns" and
           "(set W) \<inter> D0 = {}" and
           "U0 \<noteq> {}" and
@@ -636,13 +755,12 @@ lemma passification_block_lemma_aux:
                  (\<forall>ns'. s' = Normal ns' \<longrightarrow> (su = Normal u \<and> nstate_rel \<Lambda> \<Lambda>' (update_nstate_rel R Q) ns' u)))" *)
   using assms
 proof (induction arbitrary: ns U0 D0)
-  case (PAssignNormal R e1 e2 W x1 x2 Q cs1 cs2)
-  (* TODO: share proof with case PSync *)
+case (PAssignNormal R R_old e1 e2 W x1 x2 Q cs1 cs2)  (* TODO: share proof with case PSync *)
   hence "x2 \<notin> D0" and "rel_const_correct \<Lambda> R ns" by (auto simp: rel_well_typed_def)
   from \<open>A,M,\<Lambda>,\<Gamma>,\<Omega> \<turnstile> \<langle>Assign x1 e1 # cs1,Normal ns\<rangle> [\<rightarrow>] s'\<close> obtain v1 \<tau>
     where RedE1:"A,\<Lambda>,\<Gamma>,\<Omega> \<turnstile> \<langle>e1,ns\<rangle> \<Down> v1" and LookupX1:"lookup_var_ty \<Lambda> x1 = Some \<tau>" and 
                 TyV1:"type_of_val A v1 = instantiate \<Omega> \<tau>" by (meson RedCmdListCons_case single_assign_reduce_2)
-  with expr_rel_same_set[OF \<open>expr_rel R e1 e2\<close> _ \<open>rel_const_correct \<Lambda> R ns\<close> \<open>nstate_rel_states \<Lambda> \<Lambda>' R ns U0\<close>]
+  with expr_rel_same_set[OF \<open>expr_rel R R_old (snd \<Lambda>) e1 e2\<close> _ \<open>rel_const_correct \<Lambda> R ns\<close> \<open>nstate_rel_states \<Lambda> \<Lambda>' R ns U0\<close> \<open>nstate_old_rel_states \<Lambda> \<Lambda>' R_old ns U0\<close>]
   have RedE2:"\<forall>u\<in>U0. A, \<Lambda>',\<Gamma>,\<Omega> \<turnstile> \<langle>e2,u\<rangle> \<Down> v1" by blast  
   from LookupX1 have LookupX2:"lookup_var_ty \<Lambda>' x2 = Some \<tau>" using \<open>type_rel \<Lambda> \<Lambda>' ((x1, (Inl x2)) # Q)\<close> by (simp add: type_rel_def)
   let ?U1 = "(set_red_cmd A M \<Lambda>' \<Gamma> \<Omega> (Assume ((Var x2) \<guillemotleft>Eq\<guillemotright> e2)) U0)"
@@ -654,8 +772,10 @@ proof (induction arbitrary: ns U0 D0)
   have U1Dep: "dependent A \<Lambda>' \<Omega> ?U1Normal (D0 \<union> {x2})" using \<open>x2 \<notin> D0\<close> \<open>dependent A \<Lambda>' \<Omega> U0 D0\<close> RedE2    
     by (blast dest:  assume_assign_dependent)
     have RelStates: "nstate_rel_states \<Lambda> \<Lambda>' (R(x1 \<mapsto> (Inl x2))) (update_var \<Lambda> ns x1 v1) ?U1Normal"
-      using \<open>nstate_rel_states \<Lambda> \<Lambda>' R ns U0\<close> \<open>expr_rel R e1 e2\<close> \<open>rel_const_correct \<Lambda> R ns\<close> RedE1
+      using \<open>nstate_rel_states \<Lambda> \<Lambda>' R ns U0\<close> \<open>nstate_old_rel_states \<Lambda> \<Lambda>' R_old ns U0\<close> \<open>expr_rel R R_old (snd \<Lambda>) e1 e2\<close> \<open>rel_const_correct \<Lambda> R ns\<close> RedE1
       by (blast dest: assume_assign_nstate_rel)
+    have RelOldStates: "nstate_old_rel_states \<Lambda> \<Lambda>' R_old (update_var \<Lambda> ns x1 v1) ?U1Normal"
+      using \<open>nstate_old_rel_states \<Lambda> \<Lambda>' R_old ns U0\<close> U1Sub 
   from \<open>distinct (x2 # W)\<close> \<open>set (x2 # W) \<inter> D0 = {}\<close> have "distinct W" and "set W \<inter> (D0 \<union> {x2}) = {}" by auto
   from \<open>A,M,\<Lambda>,\<Gamma>,\<Omega> \<turnstile> \<langle>Assign x1 e1 # cs1,Normal ns\<rangle> [\<rightarrow>] s'\<close> have RedCs1:\<open>A,M,\<Lambda>,\<Gamma>,\<Omega> \<turnstile> \<langle>cs1, Normal (update_var \<Lambda> ns x1 v1)\<rangle> [\<rightarrow>] s'\<close>
     by (metis RedCmdListCons_case RedE1 expr_eval_determ(1) single_assign_cases)
